Rename 'wf' to 'wf_ex'
- There is a new definition of 'wf' which takes all arguments.

App/Lib/NatRangeIterator/Spec.v
@@ -8,10 +8,15 @@ Import ObjectOrientedNotations.
 Section Specs.
 Open Scope oo_scope.
 
-Definition wf (var : tm) (st : state) : Prop :=
+Definition wf_ex (var : tm) (st : state) : Prop :=
   exists n ref at_start count first,
       var = tvar n
   /\  read_sk_hd n st = tref ref
+  /\  read_sr ref st = tcl "NatRangeIterator" <(tbool at_start, tnat count, tnat first)>.
+
+Definition wf : Prop :=
+  forall var ref st at_start count first,
+      read_sk_hd var st = tref ref
   /\  read_sr ref st = tcl "NatRangeIterator" <(tbool at_start, tnat count, tnat first)>.
 
 Variable step : step_relation.
@@ -24,24 +29,24 @@ Notation "t1 '/' st1 '==>*' t2 '/' st2" := (multi step (pair t1 st1) (pair t2 st
 
 Definition get_at_start__returns_tbool : Prop :=
   forall v x st st',
-  wf x st ->
+  wf_ex x st ->
   value v ->
   (x # "get_at_start"|()|) / st ==>* v / st' ->
   exists b, v = tbool b.
 
 Definition get_at_start__terminates : Prop :=
   forall x st,
-  wf x st ->
+  wf_ex x st ->
   term_terminates step (x # "get_at_start"|()|) st.
 
 Definition get_at_start__deterministic : Prop :=
   forall x st,
-  wf x st ->
+  wf_ex x st ->
   term_deterministic step (x # "get_at_start"|()|) st.
 
 Definition get_at_start__preserves_state : Prop :=
   forall x st,
-  wf x st ->
+  wf_ex x st ->
   term_preserves_state step (x # "get_at_start"|()|) st.
 
 End Specs.
