App/Feasibility.v
@@ -46,16 +46,16 @@ Proof.
 Close Scope state_scope.
 Open Scope string_scope.
 
-Ltac expand_wf :=
+Ltac expand_wf_ex :=
   match goal with
-  | H: wf _ _ |- _ => destruct H as [n [ref [at_start [count [first [Hvar [Hsk Hsr]]]]]]]
+  | H: wf_ex _ _ |- _ => destruct H as [n [ref [at_start [count [first [Hvar [Hsk Hsr]]]]]]]
   end.
 
 Theorem off__no_side_effects:
-  Iterator.Spec.off__no_side_effects step NatRangeIterator.Spec.wf.
+  Iterator.Spec.off__no_side_effects step NatRangeIterator.Spec.wf_ex.
 Proof.
   unfold off__no_side_effects.
-  intros. expand_wf. subst x.
+  intros. expand_wf_ex. subst x.
   destruct st as [sk csk sr] eqn:Hst.
   destruct sk; try solve [destruct n; inversion Hsk].
   simpl in Hsk, Hsr.
@@ -65,5 +65,4 @@ Proof.
     repeat split.
       repeat reduce.
   Abort.
-
 
